# baseURI: http://w3id.org/abdn/socialmedia/prism#

@prefix : <http://w3id.org/abdn/socialmedia/prism#> .
@prefix prism: <http://w3id.org/abdn/socialmedia/prism#> .
@prefix dc: <http://purl.org/dc/elements/1.1/> .
@prefix dbr: <http://dbpedia.org/resource/> .
@prefix owl: <http://www.w3.org/2002/07/owl#> .
@prefix rdf: <http://www.w3.org/1999/02/22-rdf-syntax-ns#> .
@prefix var: <http://openprovenance.org/var#> .
@prefix xml: <http://www.w3.org/XML/1998/namespace> .
@prefix xsd: <http://www.w3.org/2001/XMLSchema#> .
@prefix foaf: <http://xmlns.com/foaf/0.1/> .
@prefix prov: <http://www.w3.org/ns/prov#> .
@prefix rdfs: <http://www.w3.org/2000/01/rdf-schema#> .
@prefix sioc: <http://rdfs.org/sioc/ns#> .
@prefix skos: <http://www.w3.org/2004/02/skos/core#> .
@prefix tmpl: <http://openprovenance.org/tmpl#> .
@prefix vargen: <http://openprovenance.org/vargen#> .
@prefix ns1: <http://web.resource.org/cc/> .


prism:
  rdf:type owl:Ontology ;
  rdfs:label "The Provenance of Research Involving Social Media ontology";
  dc:title "The Provenance of Research Involving Social Media ontology"^^xsd:string ;	
  dc:description """This ontology is designed to capture provenance meta-data describing the use of social media data in research projects."""@en;
  rdfs:comment """This ontology is designed to capture provenance meta-data describing the use of social media data in research projects."""@en;
  dc:creator "David Corsar"^^xsd:string ;
  dc:creator "Milan Markovic"^^xsd:string ;
  dc:rights "Copyright Â© 2015 University of Aberdeen"^^xsd:string ;
  owl:versionInfo "Revision: 0.1"^^xsd:string ;
  ns1:license <http://creativecommons.org/licenses/by-sa/3.0/> .
  
  	

_:genid31 a owl:Restriction ;
	owl:onProperty prov:used ;
	owl:allValuesFrom dbr:dataset .
	
prism:analysisMethodUsed a owl:ObjectProperty;
   rdfs:label "analysis method used";
   rdfs:comment """Relationship between a data analysis activity and the analysis method used."""@en.

_:genid32 a owl:Restriction ;
		owl:onProperty prism:analysisMethodUsed ;
		owl:allValuesFrom prism:DataAnalysisMethod .

prism:DataAnalysisMethod a owl:Class;
rdfs:label "Data analysis method";
rdfs:comment """A method utilised to analyse data."""@en.		
		
prism:usedDataFrom a owl:ObjectProperty. 

_:genid33 a owl:Restriction ;
	owl:onProperty prism:usedDataFrom ;
	owl:allValuesFrom prism:DataPreparationActivity .		
	
prism:DataAnalysisActivity a owl:Class; rdfs:subClassOf  _:genid31, _:genid32, _:genid33 ;
rdfs:label "Data analysis activity";
rdfs:comment """The activity of performing some form of data analysis"""@en.		

prism:collectedFromService a owl:DatatypeProperty;
rdfs:label "collected From Service";
rdfs:comment """Relationship between a dataset and a service/website that the data was collected from."""@en.		

prism:collectedUsing a owl:ObjectProperty; rdfs:range prism:DataCollectionTool;
rdfs:label "collected Using";
rdfs:comment """Relationship between a dataset and a tool that was used to collect the data."""@en.		

prism:DataCollectionTool a owl:Class;
   rdfs:label "Data Collection Tool";
   rdfs:comment """A (software) tool used to collect data."""@en.		

prism:dataCollectionStarted  a owl:DatatypeProperty; rdfs:range xsd:date ;   
   rdfs:label "data Collection Started";
   rdfs:comment """The date that the activity of collected data started."""@en.

prism:dataCollectionEnded  a owl:DatatypeProperty; rdfs:range xsd:date;
   rdfs:label "data Collection Ended";
   rdfs:comment """The date that the activity of collected data ended."""@en.	

prism:DataCollectionActivity a owl:Class; rdfs:subClassOf _:genid24, _:genid25;
   rdfs:label "Data Collection Activity";
   rdfs:comment """The activity of collecting data."""@en.		

_:genid24 a owl:Restriction ;
	owl:onProperty prism:dataCollectionEnded ;
	owl:qualifiedCardinality "1"^^xsd:nonNegativeInteger ;
	owl:onDataRange owl:rational .

_:genid25 a owl:Restriction ;
	owl:onProperty prism:dataCollectionStarted ;
	owl:qualifiedCardinality "1"^^xsd:nonNegativeInteger ;
	owl:onDataRange owl:rational .	
	
	
_:genid11 a owl:Restriction ;
	owl:onProperty prov:used ;
	owl:allValuesFrom dbr:dataset .
	
_:genid12 a owl:Restriction ;
	owl:onProperty prism:preparationMethodUsed ;
	owl:allValuesFrom prism:DataPreparationMethod .	
	
prism:DataPreparationActivity a owl:Class; rdfs:subClassOf  _:genid11, _:genid12 ;
   rdfs:label "Data Preparation Activity";
   rdfs:comment """The activity of preparing data, typically before or in-order-to perform some analysis."""@en.		

prism:preparationMethodUsed a owl:DatatypeProperty;
   rdfs:label "preparation Method Used";
   rdfs:comment """Relationship between a data preparation activity and the preparation method/technique used."""@en.	

prism:DataPreparationMethod a owl:Class ;
   rdfs:label "Data Preparation Method";
   rdfs:comment """A method/technique used to prepare data in some way for analysis."""@en.		

prism:trimLeadingTrailingWhitespace 
    rdf:type prism:DataPreparationMethod;
	rdfs:label "Trim leading and trailing whitespace" ;
	skos:prefLabel "Trim leading and trailing whitespace" ;
	rdfs:comment """Data preparation method in which leading and trailing whitespace are removed from a piece of text.  Based on transformation of the same label in OpenRefine."""@en.
	
prism:collapseConsecutiveWhitespace 
    rdf:type prism:DataPreparationMethod;
	rdfs:label "Collapse consecutive whitespace";
	skos:prefLabel "Collapse consecutive whitespace" ;
	rdfs:comment """Data preparation method in which multiple whitespace characters are reduced to a single character.   Based on transformation of the same label in OpenRefine."""@en.
		
prism:unescapeHtmlEntities 
    rdf:type prism:DataPreparationMethod;
	rdfs:label "Unescape HTML entities" ;
	skos:prefLabel "Unescape HTML entities" ;
	rdfs:comment """Data preparation method in which escaped HTML characters (e.g. &amp;amp;) are unescaped (e..g back to &amp;).   Based on transformation of the same label in OpenRefine."""@en.
	
	
prism:toTitlecase 
    rdf:type prism:DataPreparationMethod;
	rdfs:label  "Convert text to titlecase";
	skos:prefLabel "Convert text to titlecase";
	rdfs:comment """Data preparation method in which text is converted to title case.   Based on transformation of the same label in OpenRefine."""@en.
	

prism:toUppercase 
    rdf:type prism:DataPreparationMethod;
	rdfs:label "Convert text to uppercase";
	skos:prefLabel "Convert text to uppercase";
	rdfs:comment """Data preparation method in which text is converted to uppercase.   Based on transformation of the same label in OpenRefine."""@en.
		

prism:toLowercase 
    rdf:type prism:DataPreparationMethod;
	rdfs:label "Convert text to lowercase";
	skos:prefLabel "Convert text to lowercase";	
	rdfs:comment """Data preparation method in which text is converted to lowercase.   Based on transformation of the same label in OpenRefine."""@en.


prism:toNumber 
    rdf:type prism:DataPreparationMethod;
	rdfs:label  "Convert text to number";
	skos:prefLabel "Convert text to number";
	rdfs:comment """Data preparation method in which the type of a datum is changed from text to number.   Based on transformation of the same label in OpenRefine."""@en.
	
	
prism:toDate 
    rdf:type prism:DataPreparationMethod;
	rdfs:label "Convert text to  date";
	skos:prefLabel "Convert text to  date";
	rdfs:comment """Data preparation method in which the type of a datum is changed from text to date.   Based on transformation of the same label in OpenRefine."""@en.
	

prism:toText 
    rdf:type prism:DataPreparationMethod;
	rdfs:label "Convert to text";
	skos:prefLabel "Convert to text";	
	rdfs:comment """Data preparation method in which the type of a datum is changed to text.   Based on transformation of the same name in OpenRefine."""@en.

	
prism:textTransformation 
    rdf:type prism:DataPreparationMethod;
	rdfs:label "Transform text";
	skos:prefLabel "Transform text";
		rdfs:comment """Data preparation method in which text is transformed.   Based on transformation of the same name in OpenRefine."""@en.

	
prism:removeData 
    rdf:type prism:DataPreparationMethod;
	rdfs:label "Remove data";
	skos:prefLabel "Remove data";	
	rdfs:comment """Data preparation method in which data is removed from a dataset."""@en.


prism:filterData 
    rdf:type prism:DataPreparationMethod;
	rdfs:label  "Filter data";
	skos:prefLabel "Filter data";	
	rdfs:comment """Data preparation method in which a subset of a a dataset is created based on filtering data in the original."""@en.

